Approach

1. Whats the simplest possible input -> Find the Base Case
2. Play around the examples and visualize (sum(0) -> 0 , sum(1) -> 1 + sum(0), sum(2) -> 2 + sum(1))
3. Relate hard cases to simple cases -> Identify relations between previous executions
4. Generalize pattern -> n + sum(n-1) until base case
5. Write code -> sum(n) -> 0 if n=0 and n + sum(n-1)

---

1. Simplest Possible Input (Base Case):
   Perfect! Identifying the base case is crucial to ensure the recursion terminates. Ensure the base case handles edge cases effectively.

2. Play Around with Examples and Visualize:
   Visualization and testing simple examples help build confidence and prevent over-complication. Great step!

3. Relate Hard Cases to Simple Cases (Recursive Relation):
   Correct! Relating larger problems to smaller ones is key to understanding recursion.

4. Generalize the Pattern:
   This is where you build the recursive formula. Ensure the generalization is consistent with the base case and covers all inputs.

5. Write Code:
   Your example format looks great. Ensure the code aligns with the recursive relation and base case.

6. Additional Suggestion:
   Dry Run: After writing the code, dry run it with a few examples to ensure it works as intended. This can help catch edge cases or logical errors.
